a bunch of proofs in Util/ to help reason about while loops and booleans

coq-verification/src/Util/Loops.v
@@ -1,24 +1,28 @@
+Require Import Coq.Arith.PeanoNat.
 Require Import Coq.Lists.List.
+Require Import Hafnium.Util.List.
 Require Import Hafnium.Util.Tactics.
 
 Definition continue := false.
 Definition break := true.
-Definition while_loop
+Definition while_loop'
            {state : Type}
-           {max_iterations : nat} (* limit # iterations to prove termination *)
+           (max_iterations : nat) (* limit # iterations to prove termination *)
            (cond : state -> bool)
            (start : state)
            (body : state -> state * bool)
-  : state :=
-  fst (
-      fold_right
-        (fun _ (before : state * bool) =>
-           let '(s, loop_done) := before in
-           if (loop_done || negb (cond s))%bool
-           then (s, break) (* exit loop, keep old state *)
-           else body s)
-        (start, continue)
-        (seq 0 max_iterations)).
+  : state * bool :=
+  fold_right
+    (fun _ (before : state * bool) =>
+       let '(s, loop_done) := before in
+       if (loop_done || negb (cond s))%bool
+       then (s, break) (* exit loop, keep old state *)
+       else body s)
+    (start, continue)
+    (seq 0 max_iterations).
+Definition while_loop
+           {state} {max_iterations} cond start body : state :=
+  fst (@while_loop' state (S max_iterations) cond start body).
 
 Lemma while_loop_invariant {state} (P : state -> Prop) max_iterations cond body :
   forall start,
@@ -26,7 +30,7 @@ Lemma while_loop_invariant {state} (P : state -> Prop) max_iterations cond body 
     P start ->
     P (@while_loop _ max_iterations cond start body).
 Proof.
-  cbv [while_loop]. generalize (seq 0 max_iterations) as l.
+  cbv [while_loop while_loop']. generalize (seq 0 (S max_iterations)) as l.
   induction l;
     repeat match goal with
            | _ => progress cbn [fold_right fst snd]
@@ -37,4 +41,236 @@ Proof.
            | _ => inversion_bool
            | _ => solver
            end.
+Qed.
+
+Lemma while_loop'_0 {state} cond (start : state) body :
+  while_loop' 0 cond start body = (start, continue).
+Proof. reflexivity. Qed.
+
+Lemma while_loop'_step {state} max_iterations cond (start : state) body :
+  while_loop' (S max_iterations) cond start body =
+  if cond start
+  then if Bool.bool_dec (snd (body start)) continue
+       then while_loop' max_iterations cond (fst (body start)) body
+       else body start
+  else (start, break).
+Proof.
+  cbv [while_loop'].
+  rewrite seq_snoc, Nat.add_0_l, fold_right_app.
+  cbn [fold_right].
+  destruct (body start) as [s' loop_done].
+  repeat match goal with
+           | _ => progress cbn [fold_right fst snd] in *
+           | _ => progress cbv [continue break] in *
+           | _ => progress basics
+           | _ => break_match
+           | _ => inversion_bool
+           | _ => solver
+           | _ => apply fold_right_invariant;
+                    try destruct loop_done; basics; solver
+           end.
+Qed.
+
+Lemma while_loop'_failed {state} max_iterations cond body
+      (successful : state -> bool) :
+  (forall s, successful s = false -> successful (fst (body s)) = false) ->
+  forall start,
+    successful start = false ->
+    successful (fst (while_loop' max_iterations cond start body)) = false.
+Proof.
+  cbv [while_loop']. intros.
+  apply fold_right_invariant;
+    repeat match goal with
+           | _ => progress basics
+           | _ => progress cbn [fst snd]
+           | p : _ * _ |- _ => destruct p
+           | _ => break_match
+           | _ => solver
+           end.
+Qed.
+
+Definition sufficient_fuel {state} (ret : state * bool) : Prop :=
+  snd ret = break.
+Hint Unfold sufficient_fuel.
+
+Lemma while_loop'_completed {state} cond body
+      (successful : state -> bool) :
+  (forall s, successful (fst (body s)) = true -> snd (body s) = continue) ->
+  (forall s, successful s = false -> successful (fst (body s)) = false) ->
+  forall max_iterations start,
+    sufficient_fuel (while_loop' max_iterations cond start body) ->
+    successful (fst (while_loop' max_iterations cond start body)) = true ->
+    cond (fst (while_loop' max_iterations cond start body)) = false.
+Proof.
+  autounfold.
+  induction max_iterations;
+    repeat match goal with
+           | _ => progress basics
+           | _ => progress cbn [fst snd] in *
+           | _ => rewrite while_loop'_step in * by auto
+           | _ => rewrite while_loop'_0 in * by auto
+           | _ => break_match
+           | _ => inversion_bool
+           | _ => solver
+           | _ => cbv [continue break] in *; solver
+           | H : (forall s, successful (fst (body s)) = true -> snd (body s) = continue),
+                 H'' : _ |- _ => apply H in H''; solver
+           end.
+Qed.
+
+Definition is_measure {state} (measure: state -> nat) cond body : Prop :=
+  (forall s,
+      snd (body s) = continue ->
+      cond s = true ->
+      measure (fst (body s)) < measure s).
+
+Lemma while_loop'_sufficient_fuel {state} cond body measure :
+  is_measure measure cond body ->
+  forall max_iterations start,
+    measure start < max_iterations ->
+    sufficient_fuel (@while_loop' state max_iterations cond start body).
+Proof.
+  cbv [is_measure sufficient_fuel].
+  induction max_iterations;
+    repeat match goal with
+           | _ => progress basics
+           | _ => progress cbn [fst snd] in *
+           | _ => rewrite while_loop'_step in * by auto
+           | _ => rewrite while_loop'_0 in * by auto
+           | _ => break_match
+           | _ => inversion_bool
+           | _ => solver
+           | _ => destruct (snd (body start)); solver
+           | H : (forall s, snd (body s) = continue -> _ -> _ ),
+                 H' : _ |- _ => apply H in H'; try apply IHmax_iterations; solver
+           end.
+Qed.
+
+Lemma while_loop_completed {state} max_iterations cond body
+      (successful : state -> bool) measure start:
+  is_measure measure cond body ->
+  (forall s, successful (fst (body s)) = true -> snd (body s) = continue) ->
+  (forall s, successful s = false -> successful (fst (body s)) = false) ->
+  (measure start <= max_iterations) ->
+  successful (@while_loop _ max_iterations cond start body) = true ->
+  cond (@while_loop _ max_iterations cond start body) = false.
+Proof.
+  cbv [while_loop]; basics.
+  eapply while_loop'_completed; eauto; [ ].
+  eapply while_loop'_sufficient_fuel; solver.
+Qed.
+
+Lemma while_loop'_proper_cond {state} max_iterations body
+      cond cond' :
+  (forall s, cond s = cond' s) ->
+  forall start,
+    @while_loop' state max_iterations cond start body =
+    @while_loop' state max_iterations cond' start body.
+Proof.
+  intro Hcond_eq.
+  induction max_iterations; intros;
+    rewrite ?while_loop'_step, ?while_loop'_0 by auto;
+    rewrite ?Hcond_eq, ?IHmax_iterations by auto;
+    solver.
+Qed.
+
+Lemma while_loop_proper_cond {state} max_iterations body
+      cond cond' :
+  (forall s, cond s = cond' s) ->
+  forall start,
+    @while_loop state max_iterations cond start body =
+    @while_loop state max_iterations cond' start body.
+Proof. cbv [while_loop]; intros; erewrite while_loop'_proper_cond; eauto. Qed.
+
+Lemma while_loop'_increments {state} body
+      (value : state -> nat) (end_value : nat) :
+  (* the value increments will not skip over the end value *)
+  (forall s, snd (body s) = continue -> value s < end_value ->
+             value (fst (body s)) <= end_value) ->
+  forall max_iterations start,
+    sufficient_fuel
+      (while_loop' max_iterations (fun s => value s <? end_value) start body) ->
+    value start <= end_value ->
+    while_loop' max_iterations (fun s => value s <? end_value) start body =
+    while_loop' max_iterations (fun s => negb (value s =? end_value)) start body.
+Proof.
+  intro.
+  induction max_iterations;
+    repeat match goal with
+           | _ => progress basics
+           | _ => progress cbn [fst snd] in *
+           | _ => rewrite while_loop'_step in * by auto
+           | _ => rewrite while_loop'_0 in * by auto
+           | _ => break_match
+           | _ => inversion_bool
+           | _ => solver
+           end.
+Qed.
+
+Lemma while_loop_lt_is_measure {state} body
+      (value : state -> nat) (end_value : nat) :
+  (forall s, snd (body s) = continue -> value s < value (fst (body s))) ->
+  is_measure (fun s => end_value - value s) (fun s => value s <? end_value) body.
+Proof.
+  cbv [is_measure];
+    repeat match goal with
+           | _ => progress basics
+           | |- _ <-> _ => split
+           | |- _ = false => apply Nat.ltb_ge
+           | _ => inversion_bool
+           | _ => solver
+           | H : (forall s, snd (body s) = continue -> _ ),
+                 H' : _ |- _ => apply H in H'; solver
+           end.
+Qed.
+
+(* If a while loop's termination condition is that a particular measure of the
+   state passes a goal value, and the measure is incremented such that the goal
+   value will not be skipped over, it is equivalent to encode the while loop as
+   terminating when the state value equals the goal value, not when it's greater
+   than or equal. This is useful because it lets us declare that, when the loop
+   terminates, the final state has the exact goal value. *)
+Lemma while_loop_increments {state} max_iterations body
+      (value : state -> nat) (end_value : nat) :
+  (* the value increments monotonically increase *)
+  (forall s, snd (body s) = continue -> value s < value (fst (body s))) ->
+  (* the value increments will not skip over the end value *)
+  (forall s, snd (body s) = continue -> value s < end_value ->
+             value (fst (body s)) <= end_value) ->
+  forall start,
+    value start <= end_value ->
+    end_value - value start <= max_iterations ->
+    @while_loop _ max_iterations (fun s => value s <? end_value) start body =
+    @while_loop _ max_iterations (fun s => negb (value s =? end_value)) start body.
+Proof.
+  cbv [while_loop]; intros. apply f_equal.
+  eapply while_loop'_increments; eauto; [ ].
+  eapply while_loop'_sufficient_fuel;
+    eauto using while_loop_lt_is_measure;
+    solver.
+Qed.
+
+(* puts [while_loop_increments] and [while_loop_completed] together to prove that
+   the final "value" of the loop state will be exactly equal to the end value. *)
+Lemma while_loop_end_exact {state} max_iterations body
+      (successful : state -> bool) (value : state -> nat) (end_value : nat) :
+  (forall s, successful (fst (body s)) = true -> snd (body s) = continue) ->
+  (forall s, successful s = false -> successful (fst (body s)) = false) ->
+  (forall s, snd (body s) = continue -> value s < value (fst (body s))) ->
+  (forall s, snd (body s) = continue -> value s < end_value ->
+             value (fst (body s)) <= end_value) ->
+  forall start,
+    value start <= end_value ->
+    end_value - value start <= max_iterations ->
+    successful (@while_loop _ max_iterations (fun s => value s <? end_value) start body) = true ->
+    value (@while_loop _ max_iterations (fun s => value s <? end_value) start body) = end_value.
+Proof.
+  intros. rewrite while_loop_increments in * by auto.
+  match goal with
+  | H : successful _ = true |- _ =>
+    eapply while_loop'_completed in H; eauto
+  end; [ repeat inversion_bool; solver | ].
+  rewrite <-while_loop'_increments; eauto;
+    eapply while_loop'_sufficient_fuel;
+    eauto using while_loop_lt_is_measure; solver.
 Qed.
